tmp on mem_grow.....

theories/iris.v
@@ -193,8 +193,6 @@ Inductive reduce_simple : list administrative_instruction -> list administrative
     app_binop op v1 v2 = None ->
     reduce_simple [::AI_basic (BI_const v1); AI_basic (BI_const v2); AI_basic (BI_binop t op)] [::AI_trap]
  *)
-Print binop.
-
 Inductive pure_reduce : host_state -> store_record -> list host_value -> host_expr ->
                         host_state -> store_record -> list host_value -> host_expr -> Prop :=
 (* TODO: basic exprs -- arith ops, list ops left *)
@@ -466,6 +464,10 @@ Inductive pure_reduce : host_state -> store_record -> list host_value -> host_ex
       mem_grow m n = Some m' ->
       s' = {|s_funcs := s.(s_funcs); s_tables := s.(s_tables); s_mems := list_insert mn m' s.(s_mems); s_globals := s.(s_globals) |} ->
       pure_reduce hs s locs (HE_wasm_memory_grow idm n) hs s' locs (HE_value (HV_wasm_value (VAL_int32 (Wasm_int.int_of_Z i32m (Z.of_N (mem_size m'))))))
+  (* allows memory_grow to fail nondeterministically *)
+  | pr_memory_grow_fail_nondet:
+    forall hs s locs idm n,
+      pure_reduce hs s locs (HE_wasm_memory_grow idm n) hs s locs (HE_value (HV_trap))
   | pr_globals_create:
     forall hs s locs s' g n,
       s' = {|s_funcs := s.(s_funcs); s_tables := s.(s_tables); s_mems := s.(s_mems); s_globals := s.(s_globals) ++ [::g] |} ->
@@ -2190,6 +2192,149 @@ Qed.
       mem_grow m n = Some m' ->
       s' = {|s_funcs := s.(s_funcs); s_tables := s.(s_tables); s_mems := list_insert mn m' s.(s_mems); s_globals := s.(s_globals) |} ->
       pure_reduce hs s locs (HE_wasm_memory_grow idm n) hs s' locs (HE_value (HV_wasm_value (VAL_int32 (Wasm_int.int_of_Z i32m (Z.of_N (mem_size m'))))))
+ *)
+
+Axiom mem_length_divisible: forall m,
+  (((mem_length m) `div` page_size) * page_size)%N = mem_length m.
+
+Lemma mem_grow_size m n m':
+  mem_grow m n = Some m' ->
+  mem_size m' = (mem_size m + n)%N.
+Proof.
+  unfold mem_grow, mem_size, mem_length, memory_list.mem_length => //=.
+  move => H.
+  destruct (mem_max_opt m) in H => //=.
+  - destruct (_ <=? n0)%N => //=.
+    inversion H; subst; clear H => //=.
+    rewrite app_length.
+    rewrite repeat_length.
+    rewrite Nat2N.inj_add.
+    rewrite N2Nat.id.
+    (* lia doesn't resolve (a+b*c)/c to a/c+b, because N does not have this lemma on the right
+       side... *)
+    rewrite N.add_comm.
+    rewrite N.div_add_l => //.
+    lia.
+  - inversion H; subst; clear H => //=.
+    rewrite app_length.
+    rewrite repeat_length.
+    rewrite Nat2N.inj_add.
+    rewrite N2Nat.id.
+    rewrite N.add_comm.
+    rewrite N.div_add_l => //.
+    lia.
+Qed.
+
+Definition mem_grow_appendix (m:memory) (mn: nat) (n:N) : gmap (N*N) byte := list_to_map (imap (fun i x => ((N.of_nat mn, ((N.of_nat i) + (mem_size m) * page_size)%N), x)) (repeat #00 (N.to_nat (n * page_size)))).
+
+Lemma gmap_of_memory_grow m n m' mn mems:
+  mem_grow m n = Some m' ->
+  (mem_grow_appendix m mn n) ∪ gmap_of_memory mems =
+  gmap_of_memory (<[ mn := m' ]> mems).
+Proof.
+  move => Hmemgrow.
+  apply map_eq.
+  move => [i j].
+  unfold gmap_of_memory, mem_grow_appendix.
+  rewrite gmap_of_list_2d_lookup.
+  rewrite list_lookup_fmap.
+  destruct (_ !! N.to_nat i) eqn:Hmemlookup => //=.
+  assert (N.to_nat i < length mems) as HLen.
+  {
+    apply lookup_lt_Some in Hmemlookup.
+    by rewrite insert_length in Hmemlookup.
+  }
+  - destruct (decide (mn = N.to_nat i)); subst.
+    + rewrite list_lookup_insert in Hmemlookup => //.
+      inversion Hmemlookup; subst; clear Hmemlookup => //=.
+Admitted.
+
+Lemma wp_memory_grow s E idm mn n:
+  idm ↦ₕ (HV_wov (WOV_memoryref (Mk_memidx mn)))
+  ⊢
+  (WP HE_wasm_memory_grow idm n @ s; E
+  {{ fun v => match v with
+           | HV_wasm_value (VAL_int32 v') => ∃ (new_sz:N), (⌜ v' = Wasm_int.int_of_Z i32m (Z.of_N new_sz) ⌝ ∗ ∀ (i:N), ⌜ (i < new_sz * page_size)%N ⌝ -∗ ⌜ ((i + n * page_size)%N >= new_sz * page_size)%N ⌝  -∗ (N.of_nat mn) ↦₃[ i ] #00)
+           | HV_trap => True
+           | _ => False     
+           end
+  }})%I.
+Proof.
+  iIntros "Hmemref".
+  iApply wp_lift_atomic_step => //.
+  iIntros (σ1 ns κ κs nt) "Hσ !>".
+  destruct σ1 as [[hs ws] locs].
+  iDestruct "Hσ" as "[Hhs [? [? [? [Hwm ?]]]]]".
+  iDestruct (gen_heap_valid with "Hhs Hmemref") as "%Hmemref".
+  iSplit.
+  - iPureIntro.
+    destruct s => //.
+    apply hs_red_equiv.
+    repeat eexists.
+    by eapply pr_memory_grow_fail_nondet; eauto.
+  - iIntros "!>" (e2 [[hs' ws'] locs'] efs HStep).
+    inv_head_step; last by iFrame.
+    iMod (gen_heap_alloc_big with "Hwm") as "[Hwm [Hmembytes Htoken]]".
+    {
+      instantiate (1 := mem_grow_appendix m mn n).
+      unfold mem_grow_appendix.
+      apply map_disjoint_spec.
+      move => [i j] x y Hlookup1 Hlookup2.
+      unfold gmap_of_memory in Hlookup2.
+      resolve_finmap.
+      + rewrite gmap_of_list_2d_lookup in Hlookup2.
+        rewrite Nat2N.id in Hlookup2.
+        destruct ((_ <$> _) !! mn) eqn: HContra => //.
+        rewrite list_lookup_fmap in HContra.
+        rewrite H3 in HContra.
+        simpl in HContra.
+        inversion HContra; subst; clear HContra.
+        assert (Some y = None) => //.
+        rewrite - Hlookup2. clear Hlookup2.
+        apply lookup_ge_None.
+        unfold memory_to_list, mem_size.
+        rewrite mem_length_divisible.
+        unfold mem_length, memory_list.mem_length.
+        lia.
+      + assert (x1 = x3); first lia.
+        subst.
+        rewrite Helem0 in Helem.
+        by inversion Helem.
+      + apply nodup_imap_inj1.
+        move => n1 n2 t1 t2 Heq.
+        inversion Heq.
+        lia.
+    }
+    iModIntro. iFrame.
+    iSplitL "Hwm".
+    + by erewrite gmap_of_memory_grow.
+    + iSplit => //.
+      iExists (mem_size m').
+      iSplit => //.
+      iIntros (i) "%Hub %Hlb".
+      iDestruct (big_sepM_lookup with "Hmembytes") as "Hni" => //.
+      apply elem_of_list_to_map; resolve_finmap.
+      * assert (x0 = x2); first lia.
+        subst.
+        rewrite Helem0 in Helem.
+        by inversion Helem.
+      * apply nodup_imap_inj1.
+        move => n1 n2 t1 t2 Heq.
+        inversion Heq.
+        lia.
+      * apply elem_of_lookup_imap.
+        exists (N.to_nat (N.sub i (mem_size m * page_size))), #00.
+        apply mem_grow_size in H7.
+        rewrite H7 in Hlb.
+        assert (i >= (mem_size m * page_size))%N; first lia.
+        split => //.
+        -- repeat f_equal.
+           rewrite N2Nat.id.
+           lia.
+        -- apply repeat_lookup.
+           lia.          
+Qed.
+(*
   | pr_globals_create:
     forall hs s locs s' g n,
       s' = {|s_funcs := s.(s_funcs); s_tables := s.(s_tables); s_mems := s.(s_mems); s_globals := s.(s_globals) ++ [::g] |} ->
